WIP

src/example/LockClientSC.v
@@ -10,12 +10,18 @@ From Ordinal Require Export ClassicalHessenberg.
 
 Set Implicit Arguments.
 
+Section INIT.
 
-Module ClientImpl.
+  Definition gvs : list nat := [1].
+
   Definition loc_X := SCMem.val_ptr (0, 0).
 
   Definition const_0 := SCMem.val_nat 0.
   Definition const_42 := SCMem.val_nat 42.
+
+End INIT.
+
+Module ClientImpl.
 
   Definition thread1:
     ktree ((((@eventE void) +' cE) +' (sE unit)) +' OpenMod.callE) unit unit
@@ -53,7 +59,7 @@ Module ClientImpl.
   Definition mod: Mod.t :=
     OMod.close
       (omod)
-      (ModAdd WMem.mod FairLockW.mod)
+      (ModAdd (SCMem.mod gvs) ABSLock.mod)
   .
 
 End ClientImpl.
@@ -83,12 +89,192 @@ Module ClientSpec.
 End ClientSpec.
 
 
-From Fairness Require Import ModSim.
+
+From Fairness Require Import
+     IProp IPM Weakest ModSim PCM MonotonePCM StateRA FairRA.
 
 Section SIM.
+
+  Context `{Σ: GRA.t}.
+
+  Context `{MONORA: @GRA.inG monoRA Σ}.
+  Context `{THDRA: @GRA.inG ThreadRA Σ}.
+  Context `{STATESRC: @GRA.inG (stateSrcRA (unit)) Σ}.
+  Context `{STATETGT: @GRA.inG (stateTgtRA (unit * SCMem.t * (bool * NatMap.t unit))) Σ}.
+  Context `{IDENTSRC: @GRA.inG (identSrcRA (void)) Σ}.
+  Context `{IDENTTGT: @GRA.inG (identTgtRA (void + SCMem.val + thread_id)%type) Σ}.
+
+  Context `{OBLGRA: @GRA.inG ObligationRA.t Σ}.
+  Context `{ARROWRA: @GRA.inG (ArrowRA (void + SCMem.val + thread_id)%type) Σ}.
+  Context `{EDGERA: @GRA.inG EdgeRA Σ}.
+  Context `{ONESHOTSRA: @GRA.inG (@FiniteMap.t (OneShot.t unit)) Σ}.
+
+  Context `{MEMRA: @GRA.inG memRA Σ}.
+
+  Context `{EXCL: @GRA.inG (Excl.t unit) Σ}.
+  Context `{ONESHOTRA: @GRA.inG (OneShot.t thread_id) Σ}.
+  Context `{NATMAPRA: @GRA.inG (Auth.t (NatMapRA.t unit)) Σ}.
+  Context `{REGIONRA: @GRA.inG (Region.t (thread_id * nat)) Σ}.
+  Context `{CONSENTRA: @GRA.inG (@FiniteMap.t (Consent.t nat)) Σ}.
+  Context `{AUTHRA: @GRA.inG (Auth.t (NatMapRA.t (nat * nat))) Σ}.
+
+  Let Is: list iProp := [
+      (∃ m own ws,
+          (memory_black m)
+            ∗
+            (St_tgt (tt, m, (own, ws))));
+      ()
+
+      ((points_to loc_X const_0 ∗ OwnM (OneShot.pending thread_id 1))
+
+  Let I: list iProp := [
+      (∃ m,
+          (memory_black m)
+            **
+            (St_tgt (tt, m)));
+      (((points_to loc_l (SCMem.val_nat 0))
+          **
+          (points_to loc_f (SCMem.val_nat 0))
+          **
+          (OwnM (OneShot.pending thread_id 1)))
+       ∨
+         (∃ k,
+             (OwnM (OneShot.shot k))
+               **
+               (ObligationRA.correl_thread k 1%ord)
+               **
+               (∃ n, ObligationRA.black k n)
+               **
+               (points_to loc_l (SCMem.val_nat 1))
+               **
+               ((points_to loc_f (SCMem.val_nat 0) ** ObligationRA.pending k (/2)%Qp)
+                ∨
+                  (points_to loc_f (SCMem.val_nat 1) ** ObligationRA.shot k))))]%I.
+
+  Definition ticketlock_inv
+             (L: bool) (W: NatMap.t unit)
+             (reserved: bool)
+             (now_serving: nat) (n: nat): iProp :=
+    (wait_set_wf W n)
+      **
+      (regionl ((Nat.b2n reserved) + now_serving + n))
+      **
+      ((⌜n = 0 /\ L = false /\ reserved = false⌝ ** OwnM (Excl.just tt: Excl.t unit))
+       ∨
+         ((waiters (S ((Nat.b2n reserved) + now_serving)) n)
+            **
+            (∃ k j,
+                (ConsentP.voted_singleton k j)
+                  **
+                  (ObligationRA.correl_thread j 1%ord)
+                  **
+                  (∃ o, ObligationRA.black j o)
+                  **
+                  (((⌜L = false /\ reserved = true⌝)
+                      **
+                      (OwnM (Excl.just tt: Excl.t unit))
+                      **
+                      (waiters_tax (S ((Nat.b2n reserved) + now_serving)) n)
+                      **
+                      (ObligationRA.pending j (/2)%Qp))
+                   ∨
+                     ((⌜L = true /\ reserved = false⌝)
+                        **
+                        (ObligationRA.shot j)))))).
+
+  Definition wait_set_wf (W: NatMap.t unit) (n: nat): iProp :=
+    ((natmap_prop_sum W (fun tid _ => own_thread tid))
+       **
+       (OwnM (Auth.black (Some W: NatMapRA.t unit)))
+       **
+       (⌜NatMap.cardinal W = n⌝))
+  .
+
+  Definition regionl (n: nat): iProp :=
+    (∃ l, (Region.black l) ** (⌜List.length l = n⌝)).
+
+  Definition waiters (start n: nat): iProp :=
+    (list_prop_sum
+       (fun a => (∃ k j tid,
+                     (Region.white (start + a) (tid, k))
+                       **
+                       (OwnM (FiniteMap.singleton k (Consent.vote j (/2)%Qp)))
+                       **
+                       (ObligationRA.correl_thread j 1%ord)
+                       **
+                       (ObligationRA.pending j (/2)%Qp)
+                       **
+                       (∃ o, ObligationRA.black j o)
+                       **
+                       (FairRA.white (inl tid) (a × Ord.one)%ord)
+                       **
+                       (OwnM (Auth.white (NatMapRA.singleton tid tt: NatMapRA.t unit)))
+       ))
+       (seq 0 n))%I.
+
+  Definition waiters_tax start n: iProp :=
+    (list_prop_sum
+       (fun a => (∃ k tid,
+                     (Region.white (start + a) (tid, k))
+                       **
+                       (FairRA.white (inl tid) Ord.one)))
+       (seq 0 n))%I.
+
+  Definition ticketlock_inv
+             (L: bool) (W: NatMap.t unit)
+             (reserved: bool)
+             (now_serving: nat) (n: nat): iProp :=
+    (wait_set_wf W n)
+      **
+      (regionl ((Nat.b2n reserved) + now_serving + n))
+      **
+      ((⌜n = 0 /\ L = false /\ reserved = false⌝ ** OwnM (Excl.just tt: Excl.t unit))
+       ∨
+         ((waiters (S ((Nat.b2n reserved) + now_serving)) n)
+            **
+            (∃ k j,
+                (ConsentP.voted_singleton k j)
+                  **
+                  (ObligationRA.correl_thread j 1%ord)
+                  **
+                  (∃ o, ObligationRA.black j o)
+                  **
+                  (((⌜L = false /\ reserved = true⌝)
+                      **
+                      (OwnM (Excl.just tt: Excl.t unit))
+                      **
+                      (waiters_tax (S ((Nat.b2n reserved) + now_serving)) n)
+                      **
+                      (ObligationRA.pending j (/2)%Qp))
+                   ∨
+                     ((⌜L = true /\ reserved = false⌝)
+                        **
+                        (ObligationRA.shot j)))))).
+
   Let config := [("thread1", tt↑); ("thread2", tt↑)].
 
   Lemma client_correct:
-    UserSim.sim ClientSpec.mod ClientImpl.mod (prog2ths ClientSpec.mod config) (prog2ths ClientImpl.mod config).
-  Admitted.
+    UserSim.sim ClientSpec.mod ClientImpl.mod
+                (prog2ths ClientSpec.mod config)
+                (prog2ths ClientImpl.mod config).
+  Proof.
+    refine (@ModSim.mk _ _ nat_wf nat_wf _ _ Σ _ _ _).
+    { econs. exact 0. }
+    { i. exists (S o0). ss. }
+    { admit. }
+    { cut (forall tid,
+              (own_thread tid ** ObligationRA.duty (inl tid) []) ⊢ stsim I tid [0; 1] ibot5 ibot5 (fun r_src r_tgt => own_thread tid ** ObligationRA.duty (inl tid) [] ** ⌜r_src = r_tgt⌝) (example_spec_fun tt) (OMod.close_itree (example_omod) (SCMem.mod [1; 1]) (example_fun tt))).
+      { admit. }
+      iIntros (?) "[TH DUTY]". unfold example_spec_fun, example_fun.
+      lred. rred. rewrite close_itree_call. ss. rred.
+      iApply (stsim_yieldR with "[DUTY]"); [msubtac|iFrame|]. iIntros "DUTY _".
+      rred. unfold SCMem.cas_fun, Mod.wrap_fun. rred.
+      iopen 0 "[% [MEM ST]]" "K0".
+      iApply stsim_getR. iSplit.
+      { iFrame. }
+      rred. iApply stsim_tauR. rred.
+      unfold SCMem.cas.
+      iopen 1 "[[[POINTL POINTF] PEND]|[% H]]" "K1".
+  Abort.
+
 End SIM.
